Cleaning FMap and FSet facts.
--HG--
branch : adt

platform/cito/ConvertLabelMap.v
@@ -1,40 +1,25 @@
 Set Implicit Arguments.
 
-Require Import FMapFacts3.
-
 Require Import List.
 
-Require LabelMap.
-Module BLM := LabelMap.LabelMap.
-Module BLK := LabelMap.LabelKey.
-Require Import Equalities.
-Module BLK_as_UDT := Make_UDT BLK.
-Module Import BLMFU3 := FMapFacts3.UWFacts_fun BLK_as_UDT BLM.
-Module Import BLMFU := UWFacts.
-Module Import BLMF := WFacts.
-
-Require Import Label.
+Require Import Labels.
+Require Import LabelMap.
 Module LM := LabelMap.
-Module Label_as_UDT := Make_UDT Label_as_OT.
-Module Import LMFU3 := FMapFacts3.UWFacts_fun Label_as_UDT LM.
-Module Import LMFU := UWFacts.
-Module Import LMF := WFacts.
-Require Import ListFacts2.
-Module LF := ListFacts2.
-Module Import LFL := Make Label_as_UDT.
-
-Import LM.
-Import P.
-Import F.
+Require LabelMapFacts.
+Module LMF := LabelMapFacts.
+Require Import GLabel.
+Require Import GLabelMap.
+Import GLabelMap.
+Require Import GLabelMapFacts.
 
 Require Import ConvertLabel.
 
-Definition to_bl_pair elt (p : label * elt) := (fst p : Labels.label, snd p).
+Definition to_bl_pair elt (p : glabel * elt) := (fst p : label, snd p).
 
-Definition to_blm elt m := BLMF.to_map (List.map (@to_bl_pair _) (@elements elt m)).
+Definition to_blm elt m := LMF.of_list (List.map (@to_bl_pair _) (@elements elt m)).
 
 Module Notations.
-  Notation "m1 === m2" := (BLM.Equal m1 (to_blm m2)) (at level 70) : clm_scope.
+  Notation "m1 === m2" := (LM.Equal m1 (to_blm m2)) (at level 70) : clm_scope.
 End Notations.
 
 Section TopSection.
@@ -48,13 +33,13 @@ Section TopSection.
   Require Import Setoid.
   Require Import SetoidList.
   Require Import GeneralTactics.
-  Require Import ListFacts2.
+  Require Import ListFacts1.
 
   Set Printing Coercions.
 
-  Lemma NoDupKey_to_bl_pair_elements : forall elt m, BLMF.NoDupKey (List.map (@to_bl_pair _) (@elements elt m)).
+  Lemma NoDupKey_to_bl_pair_elements : forall elt m, LMF.NoDupKey (List.map (@to_bl_pair _) (@elements elt m)).
     intros.
-    eapply BLMFU.NoDupKey_NoDup_fst.
+    eapply LMF.NoDupKey_NoDup_fst.
     rewrite map_map.
     unfold to_bl_pair; simpl in *.
     rewrite <- map_map.
@@ -68,18 +53,18 @@ Section TopSection.
     eapply elements_3w.
   Qed.
 
-  Lemma to_blm_spec : forall elt (k : label) m, @BLM.find elt (k : Labels.label) (to_blm m) = find k m.
-    unfold to_blm, BLMF.to_map.
+  Lemma to_blm_spec : forall elt (k : glabel) m, @LM.find elt (k : label) (to_blm m) = find k m.
+    unfold to_blm, LMF.to_map.
     intros.
     eapply option_univalence; split; intros.
-    eapply BLM.find_2 in H.
-    eapply BLMF.P.of_list_1 in H.
-    eapply BLMFU.InA_eqke_In in H.
+    eapply LM.find_2 in H.
+    eapply LMF.of_list_1 in H.
+    eapply LMF.InA_eqke_In in H.
     eapply in_map_iff in H.
     openhyp.
     destruct x; simpl in *.
     unfold to_bl_pair, to_bedrock_label in *; simpl in *.
-    destruct l; simpl in *.
+    destruct g; simpl in *.
     destruct k; simpl in *.
     injection H; intros; subst.
     eapply InA_eqke_In in H0.
@@ -87,10 +72,10 @@ Section TopSection.
     eapply find_1; eauto.
     eapply NoDupKey_to_bl_pair_elements.
 
-    eapply BLM.find_1.
-    eapply BLMF.P.of_list_1.
+    eapply LM.find_1.
+    eapply LMF.of_list_1.
     eapply NoDupKey_to_bl_pair_elements.
-    eapply BLMFU.InA_eqke_In.
+    eapply LMF.InA_eqke_In.
     eapply in_map_iff.
     exists (k, v); split; eauto.
     eapply InA_eqke_In.
@@ -99,15 +84,15 @@ Section TopSection.
     eauto.
   Qed.
 
-  Lemma to_blm_no_local : forall elt s1 s2 m, @BLM.find elt (s1, Labels.Local s2) (to_blm m) = None.
-    unfold to_blm, BLMF.to_map.
+  Lemma to_blm_no_local : forall elt s1 s2 m, @LM.find elt (s1, Local s2) (to_blm m) = None.
+    unfold to_blm, LMF.to_map.
     intros.
-    eapply BLMFU3.not_in_find.
+    eapply LMF.not_in_find.
     intuition.
-    eapply BLMFU3.In_MapsTo in H.
+    eapply LMF.In_MapsTo in H.
     openhyp.
-    eapply BLMF.P.of_list_1 in H.
-    eapply BLMFU.InA_eqke_In in H.
+    eapply LMF.of_list_1 in H.
+    eapply LMF.InA_eqke_In in H.
     eapply in_map_iff in H.
     openhyp.
     unfold to_bl_pair, to_bedrock_label in *; simpl in *.
@@ -115,32 +100,32 @@ Section TopSection.
     eapply NoDupKey_to_bl_pair_elements.
   Qed.
 
-  Lemma to_blm_local_not_in : forall elt s1 s2 m, ~ @BLM.In elt (s1, Labels.Local s2) (to_blm m).
+  Lemma to_blm_local_not_in : forall elt s1 s2 m, ~ @LM.In elt (s1, Labels.Local s2) (to_blm m).
     intros.
-    eapply BLMF.P.F.not_find_in_iff.
+    eapply LMF.not_find_in_iff.
     rewrite to_blm_no_local; eauto.
   Qed.
 
-  Lemma to_blm_mapsto_iff : forall elt k (v : elt) m, BLM.MapsTo k v (to_blm m) <-> exists k' : label, MapsTo k' v m /\ k = (k' : Labels.label).
+  Lemma to_blm_mapsto_iff : forall elt k (v : elt) m, LM.MapsTo k v (to_blm m) <-> exists k' : glabel, MapsTo k' v m /\ k = (k' : label).
     split; intros.
     destruct k.
     destruct l.
     replace ((s, Labels.Global s0)) with (to_bedrock_label (s, s0)) in * by eauto.
-    eapply BLM.find_1 in H.
+    eapply LM.find_1 in H.
     rewrite to_blm_spec in H.
     eapply find_2 in H.
     eexists; eauto.
-    eapply BLMF.MapsTo_In in H.
+    eapply LMF.MapsTo_In in H.
     eapply to_blm_local_not_in in H; intuition.
     openhyp.
     subst.
-    eapply BLM.find_2.
+    eapply LM.find_2.
     rewrite to_blm_spec.
     eapply find_1; eauto.
   Qed.
 
-  Lemma to_blm_Equal : forall elt m1 m2, @BLM.Equal elt (to_blm m1) (to_blm m2) <-> m1 == m2.
-    unfold Equal, BLM.Equal.
+  Lemma to_blm_Equal : forall elt m1 m2, @LM.Equal elt (to_blm m1) (to_blm m2) <-> m1 == m2.
+    unfold Equal, LM.Equal.
     intuition.
     repeat erewrite <- to_blm_spec.
     eauto.
@@ -154,24 +139,24 @@ Section TopSection.
   Qed.
 
   Add Parametric Morphism elt : (@to_blm elt)
-      with signature Equal ==> BLM.Equal as to_blm_Equal_m.
+      with signature Equal ==> LM.Equal as to_blm_Equal_m.
     intros; eapply to_blm_Equal; eauto.
   Qed.
 
-  Lemma to_blm_In : forall elt (k : label) m, @BLM.In elt (k : Labels.label) (to_blm m) <-> In k m.
+  Lemma to_blm_In : forall elt (k : glabel) m, @LM.In elt (k : label) (to_blm m) <-> In k m.
     split; intros.
     eapply in_find_iff.
-    eapply BLMF.P.F.in_find_iff in H.
+    eapply LMF.in_find_iff in H.
     rewrite <- to_blm_spec.
     eauto.
     eapply in_find_iff in H.
-    eapply BLMF.P.F.in_find_iff.
+    eapply LMF.in_find_iff.
     rewrite to_blm_spec.
     eauto.
   Qed.
 
-  Lemma to_blm_Compat : forall elt m1 m2, @BLMFU3.Compat elt (to_blm m1) (to_blm m2) <-> Compat m1 m2.
-    unfold Compat, BLMFU3.Compat.
+  Lemma to_blm_Compat : forall elt m1 m2, @LMF.Compat elt (to_blm m1) (to_blm m2) <-> Compat m1 m2.
+    unfold Compat, LMF.Compat.
     intuition.
     repeat erewrite <- to_blm_spec.
     eapply H.
@@ -189,19 +174,19 @@ Section TopSection.
   Qed.
 
   Add Parametric Morphism elt : (@to_blm elt)
-      with signature (@Compat elt) ==> (@BLMFU3.Compat elt) as to_blm_Compat_m.
+      with signature (@Compat elt) ==> (@LMF.Compat elt) as to_blm_Compat_m.
     intros; eapply to_blm_Compat; eauto.
   Qed.
 
-  Lemma to_blm_empty : forall elt, BLM.empty elt === {}.
-    unfold Equal, BLM.Equal.
+  Lemma to_blm_empty : forall elt, LM.empty elt === {}.
+    unfold Equal, LM.Equal.
     intuition.
   Qed.
 
   Require Import GeneralTactics2.
 
-  Lemma to_blm_update : forall elt m1 m2, @BLM.Equal elt (to_blm (update m1 m2)) (BLMF.P.update (to_blm m1) (to_blm m2)).
-    unfold Equal, BLM.Equal.
+  Lemma to_blm_update : forall elt m1 m2, @LM.Equal elt (to_blm (update m1 m2)) (LMF.update (to_blm m1) (to_blm m2)).
+    unfold Equal, LM.Equal.
     intros.
     destruct y.
     destruct l; simpl.
@@ -209,28 +194,28 @@ Section TopSection.
     repeat erewrite to_blm_spec.
     destruct (In_dec m2 (s, s0)).
     rewrite update_o_2 by eauto.
-    rewrite BLMFU3.update_o_2.
+    rewrite LMF.update_o_2.
     repeat erewrite to_blm_spec.
     eauto.
     eapply to_blm_In; eauto.
     rewrite update_o_1 by eauto.
-    rewrite BLMFU3.update_o_1.
+    rewrite LMF.update_o_1.
     repeat erewrite to_blm_spec.
     eauto.
     not_not.
     eapply to_blm_In; eauto.
     repeat rewrite to_blm_no_local.
     symmetry.
-    eapply BLMFU3.not_in_find.
+    eapply LMF.not_in_find.
     intuition.
-    eapply BLMF.P.update_in_iff in H.
+    eapply LMF.update_in_iff in H.
     openhyp.
     eapply to_blm_local_not_in; eauto.
     eapply to_blm_local_not_in; eauto.
   Qed.
 
-  Lemma to_blm_diff : forall elt m1 m2, @BLM.Equal elt (to_blm (diff m1 m2)) (BLMF.P.diff (to_blm m1) (to_blm m2)).
-    unfold Equal, BLM.Equal.
+  Lemma to_blm_diff : forall elt m1 m2, @LM.Equal elt (to_blm (diff m1 m2)) (LMF.diff (to_blm m1) (to_blm m2)).
+    unfold Equal, LM.Equal.
     intros.
     destruct y.
     destruct l; simpl.
@@ -238,26 +223,26 @@ Section TopSection.
     repeat erewrite to_blm_spec.
     destruct (In_dec m2 (s, s0)).
     rewrite diff_o_none by eauto.
-    rewrite BLMFU3.diff_o_none.
+    rewrite LMF.diff_o_none.
     eauto.
     eapply to_blm_In; eauto.
     rewrite diff_o by eauto.
-    rewrite BLMFU3.diff_o.
+    rewrite LMF.diff_o.
     repeat erewrite to_blm_spec.
     eauto.
     not_not.
     eapply to_blm_In; eauto.
     repeat rewrite to_blm_no_local.
     symmetry.
-    eapply BLMFU3.not_in_find.
+    eapply LMF.not_in_find.
     intuition.
-    eapply BLMF.P.diff_in_iff in H.
+    eapply LMF.diff_in_iff in H.
     openhyp.
     eapply to_blm_local_not_in; eauto.
   Qed.
 
-  Lemma to_blm_add : forall elt (k : label) v m, @BLM.Equal elt (to_blm (add k v m)) (BLM.add (k : Labels.label) v (to_blm m)).
-    unfold Equal, BLM.Equal.
+  Lemma to_blm_add : forall elt (k : glabel) v m, @LM.Equal elt (to_blm (add k v m)) (LM.add (k : label) v (to_blm m)).
+    unfold Equal, LM.Equal.
     intros.
     destruct y.
     destruct l; simpl.
@@ -267,8 +252,8 @@ Section TopSection.
     destruct (eq_dec k (s, s0)).
     subst.
     symmetry.
-    rewrite BLMF.P.F.add_eq_o; eauto.
-    rewrite BLMF.P.F.add_neq_o.
+    rewrite LMF.add_eq_o; eauto.
+    rewrite LMF.add_neq_o.
     repeat erewrite to_blm_spec; eauto.
     not_not.
     unfold to_bedrock_label in *.
@@ -277,9 +262,9 @@ Section TopSection.
     eauto.
     repeat rewrite to_blm_no_local.
     symmetry.
-    eapply BLMFU3.not_in_find.
+    eapply LMF.not_in_find.
     intuition.
-    eapply BLMF.P.F.add_in_iff in H.
+    eapply LMF.add_in_iff in H.
     unfold to_bedrock_label in *.
     destruct k; simpl in *.
     openhyp.
