platform/cito/WordMap.v
@@ -1,66 +1,6 @@
 Set Implicit Arguments.
 
-Require Import OrderedType.
-
-Module W_as_MOT <: MiniOrderedType.
-
-  Require Import Memory.
-
-  Definition t := W.
-
-  Require Import Word.
-
-  Definition eq := @eq t.
-
-  Local Open Scope nat.
-
-  Definition lt (x y : t) := wordToNat x < wordToNat y.
-
-  Lemma eq_refl : forall x : t, eq x x.
-    unfold eq; eauto.
-  Qed.
-
-  Lemma eq_sym : forall x y : t, eq x y -> eq y x.
-    unfold eq; eauto.
-  Qed.
-
-  Lemma eq_trans : forall x y z : t, eq x y -> eq y z -> eq x z.
-    unfold eq; intuition.
-    congruence.
-  Qed.
-
-  Lemma lt_trans : forall x y z : t, lt x y -> lt y z -> lt x z.
-    unfold lt; intros; omega.
-  Qed.
-
-  Lemma lt_not_eq : forall x y : t, lt x y -> ~ eq x y.
-    unfold lt; unfold eq; intuition.
-    subst.
-    omega.
-  Qed.
-
-  Require Import WordFacts.
-
-  Definition compare : forall x y : t, Compare lt eq x y.
-    unfold lt; unfold eq.
-    intros.
-    destruct (Compare_dec.lt_eq_lt_dec (wordToNat x) (wordToNat y)).
-    destruct s.
-    econstructor 1; eauto.
-    econstructor 2; eauto.
-    eapply wordToNat_eq_eq; eauto.
-    econstructor 3; eauto.
-  Defined.
-
-End W_as_MOT.
-
-Module W_as_OT := MOT_to_OT W_as_MOT.
+Require Import WordKey.
 
 Require Import FMapAVL.
-
 Module Import WordMap := Make W_as_OT.
-
-Require Import FMapFacts.
-
-Module Import Facts := WFacts_fun W_as_OT WordMap.
-Module Import Properties := WProperties_fun W_as_OT WordMap.
