platform/cito/GLabel.v
@@ -1,0 +1,6 @@
+Set Implicit Arguments.
+
+Require Import String.
+
+Definition glabel := (string * string)%type.
+
