platform/cito/LabelMapFacts.v
@@ -1,0 +1,14 @@
+Set Implicit Arguments.
+
+Require Import LabelMap.
+Require Import Equalities.
+Module K := Make_UDT LabelKey.
+Module M := LabelMap.
+Require Import FMapFacts.
+Include (Properties M).
+Include (Facts M).
+Require Import FMapFacts1.
+Include (WFacts_fun K M).
+Include (UWFacts_fun K M).
+Require Import FMapFacts2.
+Include (UWFacts_fun K M).
