platform/cito/SetoidListFacts.v
@@ -10,7 +10,7 @@ Lemma equiv_2_trans : forall A B a b c, @equiv_2 A B a b -> equiv_2 b c -> equiv
   eapply H; eapply H0; eauto.
 Qed.
 
-Lemma InA_eq_List_In : forall elt (ls : list elt) (x : elt), InA eq x ls <-> List.In x ls.
+Lemma InA_eq_In_iff : forall elt (ls : list elt) (x : elt), InA eq x ls <-> List.In x ls.
   induction ls; simpl; intros.
   intuition.
   eapply InA_nil in H; eauto.
@@ -41,3 +41,30 @@ Qed.
 Lemma equiv_InA : forall elt (eq1 eq2 : elt -> elt -> Prop), equiv_2 eq1 eq2 -> equiv_2 (InA eq1) (InA eq2).
   unfold equiv_2; split; intros; eapply InA_weaken; eauto; intros; eapply H; eauto.
 Qed.
+
+Lemma In_InA : forall A (x : A) ls,
+  List.In x ls
+  -> InA eq x ls.
+  intros; eapply InA_eq_In_iff; eauto.
+Qed.
+
+Lemma InA_In : forall A (x : A) ls,
+  InA eq x ls ->
+  List.In x ls.
+  intros; eapply InA_eq_In_iff; eauto.
+Qed.
+
+Local Hint Constructors List.NoDup NoDupA.
+
+Lemma NoDupA_NoDup : forall A ls,
+  @NoDupA A eq ls
+  -> List.NoDup ls.
+  induction 1; intuition auto using In_InA.
+Qed.
+
+Lemma NoDup_NoDupA : forall A ls,
+  List.NoDup ls ->
+  @NoDupA A eq ls.
+  induction 1; intuition auto using InA_In.
+Qed.
+
