platform/cito/StringSetTactics.v
@@ -1,0 +1,26 @@
+Set Implicit Arguments.
+
+Require Import StringSet.
+Require Import StringSetFacts.
+Import StringSet.
+Import FSetNotations.
+
+Local Open Scope fset_scope.
+
+Ltac subset_solver :=
+  repeat
+    match goal with
+      | |- ?A <= ?A => eapply subset_refl
+      | |- empty <= _ => eapply subset_empty
+      | |- _ + _ <= _ => eapply union_subset_3
+      | |- ?S <= ?A + _ =>
+        match A with
+            context [ S ] => eapply subset_trans; [ | eapply union_subset_1]
+        end
+      | |- ?S <= _ + ?B =>
+        match B with
+            context [ S ] => eapply subset_trans; [ .. | eapply union_subset_1]
+        end
+    end.
+
+Local Close Scope fset_scope.
